Set_Graphs/Graph_Algorithms/BFS_Example.thy
@@ -1,11 +1,11 @@
-theory BFS_Example
+theory BFS_Example 
   imports BFS_Subprocedures "HOL-Data_Structures.RBT_Map"
           Directed_Set_Graphs.Pair_Graph_RBT
 begin
 
 
-definition "fold_neighb = (fold_rbt)"
-definition "fold_adj = (fold_rbt)"
+definition "fold_vset = (fold_rbt)"
+definition "fold_adjmap = (fold_rbt)"
 
 lemma prderorder_set:"set (map fst (preorder N)) = Tree2.set_tree N"
   by(induction N rule: preorder.induct)auto
@@ -13,14 +13,14 @@ lemma prderorder_set:"set (map fst (preorder N)) = Tree2.set_tree N"
 lemma preorder_witness:"set (map fst (preorder N)) = Tree2.set_tree N \<and> fold_rbt f N acc = foldr f (map fst (preorder N)) acc"
   unfolding fold_rbt_is_foldr_of_preorder prderorder_set by auto
 
-lemma rbt_fold_spec:"neighb_inv N \<Longrightarrow> \<exists>xs. set xs = Tree2.set_tree N \<and> fold_rbt f N acc = foldr f xs acc"
+lemma rbt_fold_spec:"vset_inv N \<Longrightarrow> \<exists>xs. set xs = Tree2.set_tree N \<and> fold_rbt f N acc = foldr f xs acc"
   using preorder_witness by metis
 
 
 global_interpretation bfs_subprocedures: BFS_subprocedures
 where insert = insert_rbt 
 and sel = sel 
-and neighb_empty = Leaf 
+and vset_empty = Leaf 
 and diff = diff_rbt
 and lookup = lookup 
 and empty = empty 
@@ -28,19 +28,19 @@ and delete=delete
 and isin = isin 
 and t_set=Tree2.set_tree
 and update=update 
-and adj_inv = M.invar
-and neighb_delete= delete_rbt
-and neighb_inv = neighb_inv 
+and adjmap_inv = M.invar
+and vset_delete= delete_rbt
+and vset_inv = vset_inv 
 and union=union_rbt 
 and inter=inter_rbt 
-and fold_neighb = fold_neighb
-and fold_adj=fold_adj
+and fold_vset = fold_vset
+and fold_adjmap=fold_adjmap
 and G = G for G 
 defines next_frontier = bfs_subprocedures.next_frontier
 and expand_tree = bfs_subprocedures.expand_tree
 and neighbourhood = G.neighbourhood
   apply unfold_locales
-  by (auto simp add: fold_neighb_def neighb_inv_def rbt_fold_spec neighb_inv_def fold_adj_def neighb_inv_def RBT.set_tree_union RBT.set_tree_inter RBT.set_tree_diff 
+  by (auto simp add: fold_vset_def vset_inv_def rbt_fold_spec vset_inv_def fold_adjmap_def vset_inv_def RBT.set_tree_union RBT.set_tree_inter RBT.set_tree_diff 
                 RBT.bst_union RBT.inv_union RBT.bst_inter RBT.inv_inter RBT.bst_diff RBT.inv_diff)+
 
 lemmas neighbourhood_def[unfolded G.neighbourhood_def, code] 
@@ -48,7 +48,7 @@ lemmas neighbourhood_def[unfolded G.neighbourhood_def, code]
 global_interpretation bfs: BFS
 where insert = insert_rbt 
 and sel = sel 
-and neighb_empty = Leaf 
+and vset_empty = Leaf 
 and diff = diff_rbt
 and lookup = lookup 
 and empty = empty 
@@ -56,9 +56,9 @@ and delete=delete
 and isin = isin 
 and t_set=Tree2.set_tree
 and update=update 
-and adj_inv = M.invar
-and neighb_delete=delete_rbt
-and neighb_inv = neighb_inv 
+and adjmap_inv = M.invar
+and vset_delete=delete_rbt
+and vset_inv = vset_inv 
 and union=union_rbt 
 and inter=inter_rbt
 and expand_tree = "expand_tree G"
@@ -84,7 +84,7 @@ definition "srcs =  foldr (\<lambda> x tree. insert x tree) src_list empty"
 
 value edges
 value vertices
-value "neighb_diff (nbs 1) (nbs 2)"
+value "vset_diff (nbs 1) (nbs 2)"
 value G
 value "bfs_initial_state srcs"   
 value "bfs_impl G (bfs_initial_state srcs)"
